verified counter

cfml/proofs/VerifyCounter.v
@@ -7,6 +7,31 @@ Generalizable Variables A.
 
 From Proofs Require Import Counter.
 
-(** Lazy values: a lazy value of type [a] is represented at type [unit->'a].
-    [Lazyval P f] asserts that [f] is a lazy value whose evaluation produces
-    a value satisfying the (pure) predicate [P]. *)
+
+Definition Count (n:int) (g:val) : hprop :=
+  \exists p, (p ~~> n) \*
+    \[ forall n', SPEC (g tt)
+                  PRE (p ~~> n')
+                  POST (fun r => \[r = n'] \* (p ~~> (n'+1))) ].
+
+Lemma make_counter_spec :
+  SPEC (make_counter tt)
+  PRE \[]
+  POST (fun c => c ~> Count 0).
+Proof.
+  xcf.
+  xapp;=> i.
+  xlet as;=> g Hg.
+  asserts g_spec :
+     (forall  n', SPEC (g tt)
+                    PRE (i ~~> n')
+                    POST (fun r => \[r = n'] \* (i ~~> (n'+1)))).
+  {
+    intros n'; apply Hg.
+    xapp.
+    xapp.
+    xvals*.
+  }
+  xvals*.
+  unfold Count; rewrite (@repr_eq _ _ g); xsimpl*.
+Qed.
